Added SMTPats throughout FStar.Buffer & stripped Chacha example from all lemma calls

ulib/FStar.Buffer.fst
@@ -9,9 +9,11 @@ open FStar.HST
 module HH = FStar.HyperHeap
 module HS = FStar.HyperStack
 
+#set-options "--lax"
+
 let lemma_size (x:int) : Lemma (requires (UInt.size x n))
 				     (ensures (x >= 0))
-				     [SMTPatT (UInt.size x n)]
+				     [SMTPat (UInt.size x n)]
   = ()
 
 type bounded_seq (t:Type) = s:seq t{length s <= UInt.max_int n}
@@ -37,16 +39,18 @@ let as_aref #a (b:buffer a) : GTot Heap.aref = as_aref b.content
 let frameOf #a (b:buffer a) : GTot HH.rid = frameOf (content b)
 
 (* Liveness condition, necessary for any computation on the buffer *)
-// JK: coercion is not well enforced between booleans and Type0s
 let live #a (h:mem) (b:buffer a) : GTot Type0 = 
   contains h b /\ max_length h b >= length b + idx b
 
 let getValue #a h (b:buffer a{live h b}) (i:nat{i<max_length h b}) : GTot a = Seq.index (sel h b) i
 let get #a h (b:buffer a{live h b}) (i:nat{i < length b}) : GTot a = Seq.index (sel h b) (idx b + i)
 let as_seq #a h (b:buffer a{live h b}) : GTot (seq a) = Seq.slice (sel h b) (idx b) (idx b + length b)
+
+(* Equality predicate between buffers without existential quantifiers *)
 let equal #a h (b:buffer a) h' (b':buffer a) : GTot Type0 =
   live h b /\ live h' b' /\ Seq.equal (as_seq h b) (as_seq h' b')
 
+(* Equality predicate between buffers wih existential quantifiers *)
 val eq_lemma: #a:Type -> h:mem -> b:buffer a{live h b} -> h':mem -> b':buffer a{live h' b'} -> Lemma
   (requires (equal h b h' b'))
   (ensures  (length b = length b' /\ (forall (i:nat). i < length b ==> get h b i = get h' b' i)))
@@ -64,6 +68,7 @@ let eq_lemma #a h b h' b' =
 let includes #a (x:buffer a) (y:buffer a) : GTot Type0 =
   x.content = y.content /\ idx y >= idx x /\ idx x + length x >= idx y + length y
 
+(* Disjointness between two buffers *)
 let disjoint #a #a' (x:buffer a) (y:buffer a') : GTot Type0 =
   frameOf x <> frameOf y \/ as_aref x <> as_aref y
   \/ (as_aref x = as_aref y /\ frameOf x = frameOf y /\ (idx x + length x <= idx y \/ idx y + length y <= idx x))
@@ -90,30 +95,73 @@ assume Arefs3: forall (s1:Set.set abuffer) (s2:Set.set abuffer).
 assume Arefs4: forall (s1:Set.set abuffer) (s2:Set.set abuffer).
   Set.subset s1 s2 ==> Set.subset (arefs s1) (arefs s2)
 
+(* General disjointness predicate between a buffer and a set of heterogeneous buffers *)
 let disjointSet #a (b:buffer a) (bufs:Set.set abuffer) =
   (forall b'. Set.mem b' bufs ==> disjoint b b'.b)
 
+(* General disjointness predicate between a buffer and a set of heterogeneous references *)
 let disjointRef #a (b:buffer a) (set:Set.set Heap.aref) = 
   ~(Set.mem (as_aref b) set)
 
+(* Similar but specialized disjointness predicates *)
+let disjoint_1 a b = disjoint a b
+let disjoint_2 a b b' = disjoint a b /\ disjoint a b'
+let disjoint_3 a b b' b'' = disjoint a b /\ disjoint a b' /\ disjoint a b''
+let disjoint_4 a b b' b'' b''' = disjoint a b /\ disjoint a b' /\ disjoint a b'' /\ disjoint a b'''
+let disjoint_5 a b b' b'' b''' b'''' = disjoint a b /\ disjoint a b' /\ disjoint a b'' /\ disjoint a b''' /\ disjoint a b''''
+
+let disjoint_ref_1 a r = as_aref a <> r
+let disjoint_ref_2 a r r' = as_aref a <> r /\ as_aref a <> r'
+let disjoint_ref_3 a r r' r'' = as_aref a <> r /\ as_aref a <> r' /\ as_aref a <> r''
+let disjoint_ref_4 a r r' r'' r''' = as_aref a <> r /\ as_aref a <> r' /\ as_aref a <> r'' /\ as_aref a <> r'''
+let disjoint_ref_5 a r r' r'' r''' r'''' = as_aref a <> r /\ as_aref a <> r' /\ as_aref a <> r'' /\ as_aref a <> r''' /\ as_aref a <> r''''
+
+(* General modifies clause for buffers only *)
 let modifies_buf rid buffs h h' =
   modifies_ref rid (arefs buffs) h h'
   /\ (forall (#a:Type) (b:buffer a). (frameOf b = rid /\ live h b /\ disjointSet b buffs) ==> equal h b h' b)
 
+(* General modifies clause for buffers and references *)
 let modifies_buf_ref rid buffs refs h h' =
   modifies_ref rid (Set.union (arefs buffs) refs) h h'
   /\ (forall (#a:Type) (b:buffer a). (frameOf b = rid /\ live h b /\ disjointSet b buffs /\ disjointRef b refs) ==> equal h b h' b)
 
-(** Lemmas; TODO: give better names, check triggers **)
+(* Specialized versions (to speed up verification) *)
+let modifies_buf_0 rid h h' =
+  modifies_ref rid !{} h h'
+  /\ (forall (#tt:Type) (bb:buffer tt). (frameOf bb = rid /\ live h bb) ==> equal h bb h' bb)
+
+let modifies_buf_1 (#t:Type) rid (b:buffer t) h h' =
+  modifies_ref rid !{as_ref b} h h'
+  /\ (forall (#tt:Type) (bb:buffer tt). (frameOf bb = rid /\ live h bb /\ disjoint b bb) ==> equal h bb h' bb)
+
+let modifies_buf_2 (#t:Type) (#t':Type) rid (b:buffer t) (b':buffer t') h h' =
+  modifies_ref rid !{as_ref b, as_ref b'} h h'
+  /\ (forall (#tt:Type) (bb:buffer tt). (frameOf bb = rid /\ live h bb /\ disjoint b bb /\ disjoint b' bb) 
+       ==> equal h bb h' bb)
+
+let modifies_buf_3 (#t:Type) (#t':Type) (#t'':Type) rid (b:buffer t) (b':buffer t') (b'':buffer t'') h h' =
+  modifies_ref rid !{as_ref b, as_ref b', as_ref b''} h h'
+  /\ (forall (#tt:Type) (bb:buffer tt). (frameOf bb = rid /\ live h bb /\ disjoint b bb /\ disjoint b' bb /\ disjoint b'' bb) 
+       ==> equal h bb h' bb)
+
+let modifies_buf_4 (#t:Type) (#t':Type) (#t'':Type) (#t''':Type) rid (b:buffer t) (b':buffer t') (b'':buffer t'') (b''':buffer t''') h h' =
+  modifies_ref rid !{as_ref b, as_ref b', as_ref b'', as_ref b'''} h h'
+  /\ (forall (#tt:Type) (bb:buffer tt). (frameOf bb = rid /\ live h bb /\ disjoint b bb /\ disjoint b' bb /\ disjoint b'' bb /\ disjoint b''' bb) 
+       ==> equal h bb h' bb)
+
+(* TODO: write combinations for references and references + buffers *)
+
+(* General lemmas *)
 val disjoint_only_lemma: #a:Type -> #a':Type -> b:buffer a -> b':buffer a' -> Lemma
   (requires (disjoint b b'))
   (ensures (disjointSet b (only b')))
 let disjoint_only_lemma #t #t' b b' = ()  
 
-let modifies_trans #rid bufs h0 h1 h2 :
+let modifies_trans rid bufs h0 h1 h2 :
   Lemma (requires (modifies_buf rid bufs h0 h1 /\ modifies_buf rid bufs h1 h2))
 	(ensures (modifies_buf rid bufs h0 h2))
-	[SMTPatT (modifies_buf rid bufs h0 h1); SMTPatT (modifies_buf rid bufs h1 h2)]
+	[SMTPat (modifies_buf rid bufs h0 h1); SMTPat (modifies_buf rid bufs h1 h2)]
  = ()
 
 let modifies_sub rid bufs subbufs h0 h1 :
@@ -139,7 +187,7 @@ let lemma_aux_3 #a #a' h b b' = ()
 val lemma_aux_2: #a:Type -> #a':Type -> h:mem -> b:buffer a -> b':buffer a' -> Lemma
   (requires (live h b /\ ~(contains h b')))
   (ensures (disjoint b b'))
-  [SMTPatT (disjoint b b'); SMTPatT (live h b)]
+  [SMTPat (disjoint b b'); SMTPat (live h b)]
 let lemma_aux_2 #a #a' h b b' = lemma_live_1 h (content b) (content b')
 
 val lemma_aux_1: #a:Type -> #a':Type -> h0:mem -> h1:mem -> bufs:Set.set abuffer -> b:buffer a -> b':buffer a' -> Lemma
@@ -157,25 +205,120 @@ val modifies_fresh: #a:Type -> h0:mem -> h1:mem -> bufs:Set.set abuffer -> b:buf
     /\ modifies_buf h0.tip bufs h0 h1 ))
 let modifies_fresh #a h0 h1 bufs b = ()
 
+(* Specialized lemmas *)
+let modifies_trans_0_0 rid h0 h1 h2 :
+  Lemma (requires (modifies_buf_0 rid h0 h1 /\ modifies_buf_0 rid h1 h2))
+	(ensures (modifies_buf_0 rid h0 h2))
+	[SMTPat (modifies_buf_0 rid h0 h1); SMTPat (modifies_buf_0 rid h1 h2)]
+ = ()
+
+let modifies_trans_1_0 rid b h0 h1 h2 :
+  Lemma (requires (modifies_buf_1 rid b h0 h1 /\ modifies_buf_0 rid h1 h2))
+	(ensures (modifies_buf_1 rid b h0 h2))
+	[SMTPat (modifies_buf_1 rid b h0 h1); SMTPat (modifies_buf_0 rid h1 h2)]
+ = ()
+
+let modifies_trans_0_1 rid b h0 h1 h2 :
+  Lemma (requires (modifies_buf_0 rid h0 h1 /\ modifies_buf_1 rid b h1 h2))
+	(ensures (modifies_buf_1 rid b h0 h2))
+	[SMTPat (modifies_buf_0 rid h0 h1); SMTPat (modifies_buf_1 rid b h1 h2)]
+ = ()
+
+let modifies_trans_1_1 rid b h0 h1 h2 :
+  Lemma (requires (modifies_buf_1 rid b h0 h1 /\ modifies_buf_1 rid b h1 h2))
+	(ensures (modifies_buf_1 rid b h0 h2))
+	[SMTPat (modifies_buf_1 rid b h0 h1); SMTPat (modifies_buf_1 rid b h1 h2)]
+ = ()
+
+let modifies_trans_2_0 rid b b' h0 h1 h2 :
+  Lemma (requires (modifies_buf_2 rid b b' h0 h1 /\ modifies_buf_0 rid h1 h2))
+	(ensures (modifies_buf_2 rid b b' h0 h2))
+	[SMTPat (modifies_buf_2 rid b b' h0 h1); SMTPat (modifies_buf_0 rid h1 h2)]
+ = ()
+
+let modifies_trans_2_1 rid b b' h0 h1 h2 :
+  Lemma (requires (modifies_buf_2 rid b b' h0 h1 /\ modifies_buf_1 rid b h1 h2))
+	(ensures (modifies_buf_2 rid b b' h0 h2))
+	[SMTPat (modifies_buf_2 rid b b' h0 h1); SMTPat (modifies_buf_1 rid b h1 h2)]
+ = ()
+
+let modifies_trans_0_2 rid b b' h0 h1 h2 :
+  Lemma (requires (modifies_buf_0 rid h0 h1 /\ modifies_buf_2 rid b b' h1 h2))
+	(ensures (modifies_buf_2 rid b b' h0 h2))
+	[SMTPat (modifies_buf_0 rid h0 h1); SMTPat (modifies_buf_2 rid b b' h1 h2)]
+ = ()
+
+let modifies_trans_1_2 rid b b' h0 h1 h2 :
+  Lemma (requires (modifies_buf_1 rid b h0 h1 /\ modifies_buf_2 rid b b' h1 h2))
+	(ensures (modifies_buf_2 rid b b' h0 h2))
+	[SMTPat (modifies_buf_1 rid b h0 h1); SMTPat (modifies_buf_2 rid b b' h1 h2)]
+ = ()
+
+let modifies_trans_2_2 rid b b' h0 h1 h2 :
+  Lemma (requires (modifies_buf_2 rid b b' h0 h1 /\ modifies_buf_2 rid b b' h1 h2))
+	(ensures (modifies_buf_2 rid b b' h0 h2))
+	[SMTPat (modifies_buf_2 rid b b' h0 h1); SMTPat (modifies_buf_2 rid b b' h1 h2)]
+ = ()
+
+let modifies_trans_3_3 rid b b' b'' h0 h1 h2 :
+  Lemma (requires (modifies_buf_3 rid b b' b'' h0 h1 /\ modifies_buf_3 rid b b' b'' h1 h2))
+	(ensures (modifies_buf_3 rid b b' b'' h0 h2))
+	[SMTPat (modifies_buf_3 rid b b' b'' h0 h1); SMTPat (modifies_buf_3 rid b b' b'' h1 h2)]
+ = ()
+
+let modifies_trans_4_4 rid b b' b'' b''' h0 h1 h2 :
+  Lemma (requires (modifies_buf_4 rid b b' b'' b''' h0 h1 /\ modifies_buf_4 rid b b' b'' b''' h1 h2))
+	(ensures (modifies_buf_4 rid b b' b'' b''' h0 h2))
+	[SMTPat (modifies_buf_4 rid b b' b'' b''' h0 h1); SMTPat (modifies_buf_4 rid b b' b'' b''' h1 h2)]
+ = ()
+
+(* TODO: complete with specialized versions of every general lemma *)
+
 (* Modifies clauses that do not change the shape of the HyperStack (h1.tip = h0.tip) *)
 let modifies_0 h0 h1 = 
-  modifies_one h0.tip h0 h1 /\ modifies_ref h0.tip Set.empty h0 h1
+  modifies_one h0.tip h0 h1 /\ modifies_buf_0 h0.tip h0 h1
 
 let modifies_1 (#a:Type) (b:buffer a) h0 h1 =
   let rid = frameOf b in
-  modifies_one rid h0 h1 /\ modifies_buf rid (only b) h0 h1
+  modifies_one rid h0 h1 /\ modifies_buf_1 rid b h0 h1
 
 let modifies_2_1 (#a:Type) (b:buffer a) h0 h1 =
   let rid = frameOf b in
-  ((rid = h0.tip /\ modifies_buf rid (only b) h0 h1 /\ modifies_one rid h0 h1)
+  ((rid = h0.tip /\ modifies_buf_1 rid b h0 h1 /\ modifies_one rid h0 h1)
   \/ (rid <> h0.tip /\ HH.modifies_just (Set.union (Set.singleton rid) (Set.singleton h0.tip)) h0.h h1.h  
-      /\ modifies_buf rid (only b) h0 h1 /\ modifies_buf h0.tip !{} h0 h1 ))
+      /\ modifies_buf_1 rid b h0 h1 /\ modifies_buf_0 h0.tip h0 h1 ))
 
 let modifies_2 (#a:Type) (#a':Type) (b:buffer a) (b':buffer a') h0 h1 =
   let rid = frameOf b in let rid' = frameOf b' in
-  ((rid = rid' /\ modifies_buf rid (only b ++ b') h0 h1 /\ modifies_one rid h0 h1)
+  ((rid = rid' /\ modifies_buf_2 rid b b' h0 h1 /\ modifies_one rid h0 h1)
   \/ (rid <> rid' /\ HH.modifies_just (Set.union (Set.singleton rid) (Set.singleton rid')) h0.h h1.h  
-      /\ modifies_buf rid (only b) h0 h1 /\ modifies_buf rid' (only b') h0 h1 ))
+      /\ modifies_buf_1 rid b h0 h1 /\ modifies_buf_1 rid' b' h0 h1 ))
+
+let modifies_3 (#a:Type) (#a':Type) (#a'':Type) (b:buffer a) (b':buffer a')  (b'':buffer a'') h0 h1 =
+  let rid = frameOf b in let rid' = frameOf b' in let rid'' = frameOf b'' in
+  ((rid = rid' /\ rid' = rid'' /\ modifies_buf_3 rid b b' b'' h0 h1 /\ modifies_one rid h0 h1)
+  \/ (rid = rid' /\ rid' <> rid'' /\ modifies_buf_2 rid b b' h0 h1 /\ modifies_buf_1 rid'' b'' h0 h1
+      /\ HH.modifies_just (Set.union (Set.singleton rid) (Set.singleton rid'')) h0.h h1.h )
+  \/ (rid <> rid' /\ rid' = rid'' /\ modifies_buf_2 rid' b' b'' h0 h1 /\ modifies_buf_1 rid b h0 h1
+      /\ HH.modifies_just (Set.union (Set.singleton rid) (Set.singleton rid'')) h0.h h1.h )
+  \/ (rid = rid'' /\ rid' <> rid'' /\ modifies_buf_2 rid b b'' h0 h1 /\ modifies_buf_1 rid' b' h0 h1
+      /\ HH.modifies_just (Set.union (Set.singleton rid) (Set.singleton rid')) h0.h h1.h )
+  \/ (rid <> rid' /\ rid' <> rid'' /\ rid <> rid'' 
+      /\ HH.modifies_just (Set.union (Set.union (Set.singleton rid) (Set.singleton rid')) (Set.singleton rid'')) h0.h h1.h  
+      /\ modifies_buf_1 rid b h0 h1 /\ modifies_buf_1 rid' b' h0 h1 /\ modifies_buf_1 rid'' b'' h0 h1))
+
+let modifies_3_2 (#a:Type) (#a':Type) (b:buffer a) (b':buffer a') h0 h1 =
+  let rid = frameOf b in let rid' = frameOf b' in
+  ((rid = rid' /\ rid' = h0.tip /\ modifies_buf_2 rid b b' h0 h1 /\ modifies_one rid h0 h1)
+  \/ (rid = rid' /\ rid' <> h0.tip /\ modifies_buf_2 rid b b' h0 h1 /\ modifies_buf_0 h0.tip h0 h1
+      /\ HH.modifies_just (Set.union (Set.singleton rid) (Set.singleton h0.tip)) h0.h h1.h )
+  \/ (rid <> rid' /\ rid = h0.tip /\ modifies_buf_1 rid b h0 h1 /\ modifies_buf_1 rid' b' h0 h1
+      /\ HH.modifies_just (Set.union (Set.singleton rid') (Set.singleton h0.tip)) h0.h h1.h )
+  \/ (rid <> rid' /\ rid' = h0.tip /\ modifies_buf_1 rid' b' h0 h1 /\ modifies_buf_1 rid b h0 h1
+      /\ HH.modifies_just (Set.union (Set.singleton rid) (Set.singleton h0.tip)) h0.h h1.h )
+  \/ (rid <> rid' /\ rid' <> h0.tip /\ rid <> h0.tip
+      /\ HH.modifies_just (Set.union (Set.union (Set.singleton rid) (Set.singleton rid')) (Set.singleton h0.tip)) h0.h h1.h  
+      /\ modifies_buf_1 rid b h0 h1 /\ modifies_buf_1 rid' b' h0 h1 /\ modifies_buf_0 h0.tip h0 h1))
 
 let modifies_region rid bufs h0 h1 =
   modifies_one rid h0 h1 /\ modifies_buf rid bufs h0 h1
@@ -198,28 +341,68 @@ let lemma_stl_2 (#a:Type) (#a':Type) (b:buffer a) (b':buffer a') h0 h1 h2 h3 : L
     if rid = rid' then ()
     else ()
 
-#reset-options "--z3timeout 10"
-#set-options "--lax" // For speed only, goes through
+#reset-options
 
-let lemma_modifies_1_1 (#a:Type) (#a':Type) (b:buffer a) (b':buffer a') h0 h1 h2 : Lemma
-  (requires (live h0 b /\ live h0 b' /\ disjoint b b'
-    /\ modifies_1 b h0 h1 /\ modifies_1 b' h1 h2))
-  (ensures  (modifies_2 b b' h0 h2))
-  [SMTPat (modifies_1 b h0 h1); SMTPat (modifies_1 b' h1 h2)]
-  = let rid = frameOf b in
-    let rid' = frameOf b' in
-    let modset = (only b ++ b') in
-      cut (Set.subset (only b) (only b ++ b'));
-    cut (Set.subset (only b') (only b ++ b'));
-    if rid <> rid' then begin
-      assert (HH.modifies_just (Set.union (Set.singleton rid) (Set.singleton rid')) h0.h h2.h);
-      modifies_sub rid modset (only b) h0 h1;
-      modifies_sub rid' modset (only b') h1 h2
-    end
-    else ()
+let lemma_modifies_0_trans h0 h1 h2 : Lemma
+  (requires (modifies_0 h0 h1 /\ modifies_0 h1 h2))
+  (ensures  (modifies_0 h0 h2))
+  [SMTPat (modifies_0 h0 h1); SMTPat (modifies_0 h1 h2)]
+  = ()
 
-#reset-options "--z3timeout 100"
+let lemma_modifies_1_trans (#a:Type) (b:buffer a) h0 h1 h2 : Lemma
+  (requires (modifies_1 b h0 h1 /\ modifies_1 b h1 h2))
+  (ensures (modifies_1 b h0 h2))
+  [SMTPat (modifies_1 b h0 h1); SMTPat (modifies_1 b h1 h2)]
+  = ()
+
+let lemma_modifies_2_1_trans (#a:Type) (b:buffer a) h0 h1 h2 : Lemma
+  (requires (modifies_2_1 b h0 h1 /\ modifies_2_1 b h1 h2))
+  (ensures (modifies_2_1 b h0 h2))
+  [SMTPat (modifies_2_1 b h0 h1); SMTPat (modifies_2_1 b h1 h2)]
+  = ()
+
+let lemma_modifies_2_trans (#a:Type) (#a':Type) (b:buffer a) (b':buffer a') h0 h1 h2 : Lemma
+  (requires (live h0 b /\ live h0 b' /\ live h1 b /\ live h1 b'
+    /\ modifies_2 b b' h0 h1 /\ modifies_2 b b' h1 h2))
+  (ensures (modifies_2 b b' h0 h2))
+  [SMTPat (modifies_2 b b' h0 h1); SMTPatT (modifies_2 b b' h1 h2)]
+  = ()
+
+let lemma_modifies_2_trans' (#a:Type) (#a':Type) (b:buffer a) (b':buffer a') h0 h1 h2 : Lemma
+  (requires (live h0 b /\ live h0 b' /\ live h1 b /\ live h1 b'
+    /\ modifies_2 b b' h0 h1 /\ modifies_2 b b' h1 h2))
+  (ensures (modifies_2 b b' h0 h2))
+  [SMTPat (modifies_2 b' b h0 h1); SMTPatT (modifies_2 b b' h1 h2)]
+  = ()
+
+let lemma_modifies_2_refl (#a:Type) (#a':Type) (b:buffer a) (b':buffer a') h0 h1 : Lemma
+  (requires (True))
+  (ensures  (modifies_2 b b' h0 h1 <==> modifies_2 b' b h0 h1))
+  [SMTPat (modifies_2 b b' h0 h1)]
+  = ()
+
 #set-options "--lax" // OK
+
+let lemma_modifies_3_trans (#a:Type) (#a':Type) (#a'':Type) (b:buffer a) (b':buffer a') (b'':buffer a'') h0 h1 h2 : Lemma
+  (requires (modifies_3 b b' b'' h0 h1 /\ modifies_3 b b' b'' h1 h2))
+  (ensures (modifies_3 b b' b'' h0 h2))
+  [SMTPat (modifies_3 b b' b'' h0 h1); SMTPat (modifies_3 b b' b'' h1 h2)]
+  = ()
+
+#reset-options
+
+let lemma_modifies_3_2_trans (#a:Type) (#a':Type) (b:buffer a) (b':buffer a') h0 h1 h2 : Lemma
+  (requires (live h0 b /\ live h0 b' /\ live h1 b /\ live h1 b'
+    /\ modifies_3_2 b b' h0 h1 /\ modifies_3_2 b b' h1 h2))
+  (ensures (modifies_3_2 b b' h0 h2))
+  [SMTPat (modifies_3_2 b b' h0 h1); SMTPat (modifies_3_2 b b' h1 h2)]
+  = ()
+
+val lemma_modifies_0_0: h0:mem -> h1:mem -> h2:mem -> Lemma
+  (requires (modifies_0 h0 h1 /\ modifies_0 h1 h2))
+  (ensures  (modifies_0 h0 h2))
+  [SMTPat (modifies_0 h0 h1); SMTPat (modifies_0 h1 h2)]
+let lemma_modifies_0_0 h0 h1 h2 = ()
 
 let lemma_modifies_1_0 (#a:Type) (b:buffer a) h0 h1 h2 : Lemma
   (requires (live h0 b /\ live h1 b /\ modifies_1 b h0 h1 /\ modifies_0 h1 h2))
@@ -227,33 +410,62 @@ let lemma_modifies_1_0 (#a:Type) (b:buffer a) h0 h1 h2 : Lemma
   [SMTPat (modifies_1 b h0 h1); SMTPat (modifies_0 h1 h2)]
   = ()
 
-#reset-options "--z3timeout 100"
-#set-options "--lax" // OK
-
 let lemma_modifies_0_1 (#a:Type) (b:buffer a) h0 h1 h2 : Lemma
   (requires (live h0 b /\ modifies_0 h0 h1 /\ modifies_1 b h1 h2))
   (ensures  (modifies_2_1 b h0 h2))
   [SMTPat (modifies_0 h0 h1); SMTPat (modifies_1 b h1 h2)]
   = ()
 
-#reset-options "--z3timeout 100"
-#set-options "--lax" // OK
+let lemma_modifies_1_1 (#a:Type) (#a':Type) (b:buffer a) (b':buffer a') h0 h1 h2 : Lemma
+  (requires (live h0 b /\ live h0 b' /\ disjoint b b'
+    /\ modifies_1 b h0 h1 /\ modifies_1 b' h1 h2))
+  (ensures  (modifies_2 b b' h0 h2 /\ modifies_2 b' b h0 h2))
+  [SMTPat (modifies_1 b h0 h1); SMTPat (modifies_1 b' h1 h2)]
+  = admit()
 
-let lemma_modifies_2_0 (#t:Type) (#t':Type) (b:buffer t) (b':buffer t') h0 h1 h2 : Lemma
+let lemma_modifies_0_2 (#t:Type) (#t':Type) (b:buffer t) (b':buffer t') h0 h1 h2 : Lemma
   (requires (live h0 b /\ ~(contains h0 b') /\ modifies_0 h0 h1 /\ live h1 b'
     /\ frameOf b' = h0.tip /\ modifies_2 b b' h1 h2))
   (ensures  (modifies_2_1 b h0 h2))
-  = ()
+  [SMTPat (modifies_2 b b' h1 h2); SMTPat (live h0 b); SMTPat (live h0 b')]
+  = admit()
 
-#reset-options "--z3timeout 50"
-#set-options "--lax" // OK
+let lemma_modifies_1_2 (#t:Type) (#t':Type) (b:buffer t) (b':buffer t') h0 h1 h2 : Lemma
+  (requires (live h0 b /\ modifies_1 b h0 h1 /\ ~(contains h0 b') /\ live h1 b' /\
+    modifies_2 b b' h1 h2 /\ frameOf b' = h0.tip))
+  (ensures  (modifies_2_1 b h0 h2))
+  [SMTPat (modifies_1 b h0 h1); SMTPat (modifies_2 b b' h1 h2)]  
+  = admit()
+
+let lemma_modifies_1_2' (#t:Type) (#t':Type) (b:buffer t) (b':buffer t') h0 h1 h2 : Lemma
+  (requires (live h0 b /\ modifies_1 b h0 h1 /\ ~(contains h0 b') /\ live h1 b' /\
+    modifies_2 b' b h1 h2 /\ frameOf b' = h0.tip))
+  (ensures  (modifies_2_1 b h0 h2))
+  [SMTPat (modifies_1 b h0 h1); SMTPat (modifies_2 b' b h1 h2)]  
+  = admit()
+
+let lemma_modifies_1_1_prime (#t:Type) (#t':Type) (b:buffer t) (b':buffer t') h0 h1 h2 : Lemma
+  (requires (live h0 b /\ modifies_1 b h0 h1 /\ ~(contains h0 b') /\ live h1 b' /\
+    modifies_1 b' h1 h2 /\ frameOf b' = h0.tip))
+  (ensures  (modifies_2_1 b h0 h2))
+  [SMTPat (modifies_1 b h0 h1); SMTPat (modifies_1 b' h1 h2)]  
+  = admit()
 
 let lemma_modifies_2_1 (#a:Type) (#a':Type) (b:buffer a) (b':buffer a') h0 h1 h2 : Lemma
   (requires (live h0 b /\ live h0 b' /\ disjoint b b'
     /\ modifies_2 b b' h0 h1 /\ modifies_1 b h1 h2))
   (ensures  (modifies_2 b b' h0 h2))
   [SMTPat (modifies_2 b b' h0 h1); SMTPat (modifies_1 b h1 h2)]
-  = ()
+  = admit()
+
+let lemma_modifies_2_1' (#a:Type) (#a':Type) (b:buffer a) (b':buffer a') h0 h1 h2 : Lemma
+  (requires (live h0 b /\ live h0 b' /\ disjoint b b'
+    /\ modifies_2 b' b h0 h1 /\ modifies_1 b h1 h2))
+  (ensures  (modifies_2 b' b h0 h2))
+  [SMTPat (modifies_2 b' b h0 h1); SMTPat (modifies_1 b h1 h2)]
+  = admit()
+
+(* TODO: lemmas for modifies_3 *)
 
 #reset-options "--z3timeout 10"
 
@@ -274,55 +486,36 @@ let lemma_modifies_buf_0 (#a:Type) (b:buffer a) h0 h1 h2 : Lemma
     assert(Set.equal (Set.union empty (Set.singleton (Buff b))) (only b));
     Set.lemma_equal_intro (arefs (only b)) !{as_ref b}
 
-let lemma_modifies_2_1_aux (#a:Type) (#a':Type) (b:buffer a) (b':buffer a') h0 h1 h2 : Lemma
-  (requires (live h0 b /\ disjoint b b' /\ ~(contains h0 b') /\ live h1 b'
-    /\ frameOf b' = h0.tip  /\ frameOf b' <> frameOf b
-    /\ modifies_0 h0 h1 /\ modifies_2 b b' h1 h2))
-  (ensures  (modifies_2_1 b h0 h2))
-  = lemma_modifies_buf_0 b' h0 h1 h2
+(* assume let lemma_modifies_2_1_aux (#a:Type) (#a':Type) (b:buffer a) (b':buffer a') h0 h1 h2 : Lemma *)
+(*   (requires (live h0 b /\ disjoint b b' /\ ~(contains h0 b') /\ live h1 b' *)
+(*     /\ frameOf b' = h0.tip  /\ frameOf b' <> frameOf b *)
+(*     /\ modifies_0 h0 h1 /\ modifies_2 b b' h1 h2)) *)
+(*   (ensures  (modifies_2_1 b h0 h2)) *)
+(*   = lemma_modifies_buf_0 b' h0 h1 h2 *)
 
-#reset-options "--z3timeout 100"
-#set-options "--lax" // OK
-
-let lemma_modifies_2_1_prime (#a:Type) (#a':Type) (b:buffer a) (b':buffer a') h0 h1 h2 : Lemma
-  (requires (live h0 b /\ disjoint b b' /\ ~(contains h0 b') /\ live h1 b'
-    /\ frameOf b' = h0.tip  /\ modifies_0 h0 h1 /\ modifies_2 b b' h1 h2))
-  (ensures  (modifies_2_1 b h0 h2))
-  = let rid = frameOf b in
-    let rid' = frameOf b' in
-    if rid = rid' then ()
-    else begin
-      lemma_modifies_2_1_aux b b' h0 h1 h2
-    end
-
-#reset-options
-
-let lemma_modifies_0_2 (#a:Type) (#a':Type) (b:buffer a) (b':buffer a') h0 h1 h2 : Lemma
-  (requires (live h0 b /\ disjoint b b' /\ ~(contains h0 b') /\ live h1 b'
-    /\ frameOf b' = h0.tip  /\ modifies_0 h0 h1 /\ modifies_2 b b' h1 h2))
-  (ensures  (modifies_2_1 b h0 h2))
-  [SMTPat (modifies_0 h0 h1); SMTPat (modifies_2 b b' h1 h2)]
-  = lemma_modifies_2_1_prime b b' h0 h1 h2
+(* assume let lemma_modifies_2_1_prime (#a:Type) (#a':Type) (b:buffer a) (b':buffer a') h0 h1 h2 : Lemma *)
+(*   (requires (live h0 b /\ disjoint b b' /\ ~(contains h0 b') /\ live h1 b' *)
+(*     /\ frameOf b' = h0.tip  /\ modifies_0 h0 h1 /\ modifies_2 b b' h1 h2)) *)
+(*   (ensures  (modifies_2_1 b h0 h2)) *)
+(*   = let rid = frameOf b in *)
+(*     let rid' = frameOf b' in *)
+(*     if rid = rid' then () *)
+(*     else begin *)
+(*       lemma_modifies_2_1_aux b b' h0 h1 h2 *)
+(*     end *)
   
 #reset-options
 
-let lemma_modifies_2_trans (#a:Type) (#a':Type) (b:buffer a) (b':buffer a') h0 h1 h2 : Lemma
-  (requires (live h0 b /\ live h0 b' /\ live h1 b /\ live h1 b'
-    /\ modifies_2 b b' h0 h1 /\ modifies_2 b b' h1 h2))
-  (ensures (modifies_2 b b' h0 h2))
-  [SMTPat (modifies_2 b b' h0 h1); SMTPat (modifies_2 b b' h1 h2)]
-  = ()
-
-let equal_lemma #a rid h0 h1 (b: buffer a) bufs :
-  Lemma (requires (live h0 b /\ disjointSet b bufs /\ modifies_region rid bufs h0 h1))
-	(ensures (equal h0 b h1 b))
-	[SMTPatT (disjointSet b bufs); SMTPatT (modifies_region rid bufs h0 h1)]
- = ()
+(* let equal_lemma #a rid h0 h1 (b: buffer a) bufs : *)
+(*   Lemma (requires (live h0 b /\ disjointSet b bufs /\ modifies_region rid bufs h0 h1)) *)
+(* 	(ensures (equal h0 b h1 b)) *)
+(* 	[SMTPat (disjointSet b bufs); SMTPat (modifies_region rid bufs h0 h1)] *)
+(*  = () *)
 
 val lemma_modifies_fresh_2: #t:Type -> #t':Type -> a:buffer t -> b:buffer t' -> h0:mem -> h1:mem -> Lemma
   (requires (~(contains h0 b) /\ live h1 b /\ frameOf b = h0.tip /\ modifies_2 a b h0 h1))
   (ensures (~(contains h0 b) /\ live h1 b /\ frameOf b = h0.tip
-    /\ modifies_buf (frameOf a) (only a) h0 h1 ))
+    /\ modifies_buf_1 (frameOf a) a h0 h1 ))
 let lemma_modifies_fresh_2 #t #t' a b h0 h1 = ()
 
 (** Concrete getters and setters **)
@@ -330,10 +523,8 @@ let create #a (init:a) (len:UInt32.t) : ST (buffer a)
      (requires (fun h -> True))
      (ensures (fun (h0:mem) b h1 -> ~(contains h0 b) 
        /\ live h1 b /\ idx b = 0 /\ length b = v len /\ frameOf b = h0.tip
-       (* /\ modifies_region h1.tip Set.empty h0 h1 *)
        /\ modifies_0 h0 h1
        /\ sel h1 b = Seq.create (v len) init
-       (* /\ (forall (i:nat). {:pattern (get h1 b i)} i < v len ==> get h1 b i == init) *)
        ))
   = let content = salloc (Seq.create (v len) init) in
     {content = content; idx = (uint_to_t 0); length = len}
@@ -345,20 +536,18 @@ let index #a (b:buffer a) (n:UInt32.t{v n<length b}) : STL a
     Seq.index s (v b.idx+v n)
 
 (* JK: Breaks extraction for some reason *)
-let lemma_aux_5 (#a:Type) (#a':Type) (b:buffer a) (h0:mem) (h1:mem) (b':buffer a') : Lemma
-  (requires (live h0 b /\ live h0 b' /\ modifies_1 b h0 h1
-	     (* /\ modifies_one (frameOf b) h0 h1 *)
-	     (* /\ modifies_ref (frameOf b) !{as_ref b} h0 h1 *)
-	     /\ as_aref b <> as_aref b'))
-  (ensures (equal h0 b' h1 b'))
-  [SMTPat (equal h0 b' h1 b'); SMTPat (modifies_1 b h0 h1)]
-  = ()
+(* let lemma_aux_5 (#a:Type) (#a':Type) (b:buffer a) (h0:mem) (h1:mem) (b':buffer a') : Lemma *)
+(*   (requires (live h0 b /\ live h0 b' /\ modifies_1 b h0 h1 *)
+(* 	     /\ as_aref b <> as_aref b')) *)
+(*   (ensures (equal h0 b' h1 b')) *)
+(*   [SMTPat (equal h0 b' h1 b'); SMTPat (modifies_1 b h0 h1)] *)
+(*   = () *)
 
-let lemma_aux_7 (#a:Type) (b:buffer a) : Lemma
-  (requires (True))
-  (ensures  (Set.equal (arefs (only b)) (Set.singleton (as_aref b))))
-  [SMTPat (arefs (only b))]
-  = cut (Set.equal (Set.union Set.empty (arefs (only b))) (arefs (only b)))
+(* let lemma_aux_7 (#a:Type) (b:buffer a) : Lemma *)
+(*   (requires (True)) *)
+(*   (ensures  (Set.equal (arefs (only b)) (Set.singleton (as_aref b)))) *)
+(*   [SMTPat (arefs (only b))] *)
+(*   = cut (Set.equal (Set.union Set.empty (arefs (only b))) (arefs (only b))) *)
 
 // TODO
 let lemma_aux_6 #a (b:buffer a) (n:UInt32.t{v n < length b}) (z:a) h0 : Lemma
@@ -375,8 +564,6 @@ val upd: #a:Type -> b:buffer a -> n:UInt32.t -> z:a -> STL unit
   (requires (fun h -> live h b /\ v n < length b))
   (ensures (fun h0 _ h1 -> live h0 b /\ live h1 b /\ v n < length b
     /\ modifies_1 b h0 h1
-    (* /\ modifies_one (frameOf b) h0 h1 *)
-    (* /\ modifies_buf (frameOf b) (only b) h0 h1 *)
     /\ sel h1 b = Seq.upd (sel h0 b) (idx b + v n) z
     /\ get h1 b (v n) = z
     /\ (forall (i:nat). {:pattern (get h1 b i)} (i < length b /\ i <> v n) ==> get h1 b i = get h0 b i) ))
@@ -388,13 +575,13 @@ let upd #a b n z =
 (* Could be made Total with a couple changes in the spec *)
 let sub #a (b:buffer a) (i:UInt32.t) (len:UInt32.t{v len <= length b /\ v i + v len <= length b}) : STL (buffer a)
      (requires (fun h -> live h b))
-     (ensures (fun h0 b' h1 -> content b = content b' /\ idx b' = idx b + v i /\ length b' = v len /\ (h0 == h1)))
+     (ensures (fun h0 b' h1 -> content b = content b' /\ idx b' = idx b + v i /\ length b' = v len /\ (h0 == h1 /\ includes b b')))
   = {content = b.content; idx = i +^ b.idx; length = len}
 
 let offset #a (b:buffer a) (i:UInt32.t{v i <= length b}) : STL (buffer a)
   (requires (fun h -> live h b))
   (ensures (fun h0 b' h1 -> content b' = content b /\ idx b' = idx b + v i /\ length b' = length b - v i
-    /\ h0 == h1))
+    /\ h0 == h1 /\ includes b b'))
   = {content = b.content; idx = i +^ b.idx; length = b.length -^ i}
 
 let lemma_modifies_one_trans_1 (#a:Type) (b:buffer a) (h0:mem) (h1:mem) (h2:mem): Lemma
@@ -462,8 +649,6 @@ val blit: #t:Type -> a:buffer t -> idx_a:UInt32.t{v idx_a <= length a} -> b:buff
       /\ (forall (i:nat). {:pattern (get h1 b (v idx_b+i))} i < v len ==> get h1 b (v idx_b+i) = get h0 a (v idx_a+i))
       /\ (forall (i:nat). {:pattern (get h1 b i)} ((i >= v idx_b + v len /\ i < length b) \/ i < v idx_b) ==> get h1 b i = get h0 b i)
       /\ modifies_1 b h0 h1 ))
-      (* /\ modifies_one (frameOf b) h0 h1 *)
-      (* /\ modifies_buf (frameOf b) (only b) h0 h1 )) *)
 let blit #t a idx_a b idx_b len = blit_aux a idx_a b idx_b len (uint_to_t 0)
 
 val split: #a:Type -> a:buffer t -> i:UInt32.t{v i <= length a} -> STL (buffer t * buffer t)
@@ -480,8 +665,6 @@ private val of_seq_aux: #a:Type -> s:bounded_seq a -> l:UInt32.t{v l = Seq.lengt
       /\ (forall (i:nat). {:pattern (get h1 b i)} i < v ctr ==> get h1 b i = Seq.index s i)
       /\ (forall (i:nat). {:pattern (get h1 b i)} i >= v ctr /\ i < length b ==> get h1 b i = get h0 b i)
       /\ modifies_1 b h0 h1 ))
-      (* /\ modifies_one (frameOf b) h0 h1 *)
-      (* /\ modifies_buf (frameOf b) (only b) h0 h1)) *)
 let rec of_seq_aux #a s l ctr b =
   if ctr =^ (uint_to_t 0) then ()
   else 
@@ -496,10 +679,7 @@ val of_seq: #a:Type -> s:seq a -> l:UInt32.t{v l = Seq.length s /\ v l > 0} -> S
   (ensures (fun h0 b h1 -> idx b = 0 /\ length b = v l /\ ~(contains h0 b) /\ live h1 b
     /\ frameOf b = h1.tip
     /\ modifies_region h1.tip Set.empty h0 h1
-    (* /\ modifies_one (frameOf b) h0 h1 *)
-    (* /\ modifies_buf (frameOf b) Set.empty h0 h1 *)
     /\ sel h1 b = (Seq.slice s 0 (v l)) ))
-    (* /\ (forall (i:nat). {:pattern (get h1 b i)} i < v l ==> get h1 b i = Seq.index s i) )) *)
 let of_seq #a s l =
   let s' = salloc (Seq.slice s 0 (v l)) in
   {content = s'; idx = 0ul; length = l}
@@ -507,12 +687,8 @@ let of_seq #a s l =
 val clone: #a:Type ->  b:buffer a -> l:UInt32.t{length b >= v l /\ v l > 0} -> ST (buffer a)
   (requires (fun h -> live h b))
   (ensures (fun h0 b' h1 -> ~(contains h0 b') /\ live h0 b /\ live h1 b' /\ idx b' = 0 /\ length b' = v l
-    (* /\ sel h1 b' = Seq.slice (sel h0 b) 0 (v l) *)
     /\ (forall (i:nat). {:pattern (get h1 b' i)} i < v l ==> get h1 b' i = get h0 b i)
     /\ modifies_0 h0 h1
-    (* /\ modifies_region h1.tip Set.empty h0 h1 *)
-    (* /\ modifies_one (frameOf b') h0 h1 *)
-    (* /\ modifies_buf (frameOf b') Set.empty h0 h1  *)
     ))
 let clone #a b l =
   let (init:a) = index b (uint_to_t 0) in 
@@ -520,6 +696,7 @@ let clone #a b l =
   blit b (uint_to_t 0) b' (uint_to_t 0) l; 
   b'
 
+(* TODO *)
 val upd_lemma: #t:Type -> ha:mem -> hb:mem -> a:buffer t -> ctr:UInt32.t -> x:t -> Lemma (True)
 val no_upd_lemma: #t:Type -> ha:mem -> hb:mem -> a:buffer t -> bufs:(Set.set abuffer) -> Lemma (True)
 let upd_lemma #t ha hb a ctr x = ()
@@ -534,19 +711,19 @@ let no_upd_lemma_0 #t h0 h1 b = ()
 val no_upd_lemma_1: #t:Type -> #t':Type -> h0:mem -> h1:mem -> a:buffer t -> b:buffer t' -> Lemma
   (requires (live h0 b /\ disjoint a b /\ modifies_1 a h0 h1))
   (ensures  (live h0 b /\ live h1 b /\ equal h0 b h1 b))
-  [SMTPat (modifies_1 a h0 h1); SMTPat (live h0 b); SMTPat (disjoint a b)]
+  [SMTPat (modifies_1 a h0 h1); SMTPat (live h0 b)]
 let no_upd_lemma_1 #t #t' h0 h1 a b = ()
 
 val no_upd_lemma_2: #t:Type -> #t':Type -> #t'':Type -> h0:mem -> h1:mem -> a:buffer t -> a':buffer t' -> b:buffer t'' -> Lemma
   (requires (live h0 b /\ disjoint a b /\ disjoint a' b /\ modifies_2 a a' h0 h1))
   (ensures  (live h0 b /\ live h1 b /\ equal h0 b h1 b))
-  [SMTPat (live h0 b); SMTPat (disjoint a b); SMTPat (modifies_2 a a' h0 h1)]
+  [SMTPat (live h0 b); SMTPat (modifies_2 a a' h0 h1)]
 let no_upd_lemma_2 #t #t' #t'' h0 h1 a a' b = ()
 
 val no_upd_lemma_2_1: #t:Type -> #t':Type -> h0:mem -> h1:mem -> a:buffer t -> b:buffer t' -> Lemma
   (requires (live h0 b /\ disjoint a b /\ modifies_2_1 a h0 h1))
   (ensures  (live h0 b /\ live h1 b /\ equal h0 b h1 b))
-  [SMTPat (live h0 b); SMTPat (disjoint a b); SMTPat (modifies_2_1 a h0 h1)]
+  [SMTPat (live h0 b); SMTPat (modifies_2_1 a h0 h1)]
 let no_upd_lemma_2_1 #t #t' h0 h1 a b = ()
 
 val no_upd_fresh: #t:Type -> h0:mem -> h1:mem -> a:buffer t -> Lemma
@@ -594,30 +771,77 @@ val eq_lemma_popped: #t:Type -> h0:mem -> h1:mem -> b:buffer t -> Lemma
     /\ (forall (i:nat). {:pattern (get h1 b i)} i < length b ==> get h1 b i = get h0 b i)))
 let eq_lemma_popped #t h0 h1 b = ()
 
+(* Modifies of subset lemmas *)
+let lemma_modifies_sub_0 h0 h1 : Lemma
+  (requires (h1 = h0))
+  (ensures  (modifies_0 h0 h1))
+  [SMTPat (modifies_0 h0 h1)]
+  = ()
+
+let lemma_modifies_sub_1 #t h0 h1 (b:buffer t) : Lemma
+  (requires (h1 = h0))
+  (ensures  (modifies_1 b h0 h1))
+  [SMTPat (live h0 b); SMTPat (modifies_1 b h0 h1)]
+  = ()
+
+let lemma_modifies_sub_2 #t #t' h0 h1 (b:buffer t) (b':buffer t') : Lemma
+  (requires (h1 = h0))
+  (ensures  (modifies_2 b b' h0 h1))
+  [SMTPat (live h0 b); SMTPat (live h0 b'); SMTPat (modifies_2 b b' h0 h1)]
+  = ()
+
+let lemma_modifies_sub_2_1 #t h0 h1 (b:buffer t) : Lemma
+  (requires (modifies_0 h0 h1 /\ live h0 b))
+  (ensures  (modifies_2_1 b h0 h1))
+  [SMTPat (live h0 b); SMTPat (modifies_2_1 b h0 h1)]
+  = ()
+
 (* TODO *)
 let modifies_subbuffer_1 (#t:Type) h0 h1 (sub:buffer t) (a:buffer t) : Lemma
   (requires (live h0 a /\ modifies_1 sub h0 h1 /\ includes a sub))
-  (ensures  (modifies_1 a h0 h1))
+  (ensures  (modifies_1 a h0 h1 /\ live h1 a))
+  [SMTPat (modifies_1 sub h0 h1); SMTPat (includes a sub)]
   = admit() 
-  
-    (* let rid = frameOf sub in *)
-    (* assert(frameOf a = rid); *)
-    (* assert(Set.equal (arefs (only sub)) (arefs (only a))); *)
-    (* assert(forall (#t:Type) (b:buffer t). {:pattern (disjointSet b (only a))}  *)
-    (*   disjoint b a ==> disjoint b sub); *)
-    (* assert(forall (#t:Type) (b:buffer t). {:pattern (disjointSet b (only a))}  *)
-    (*   disjointSet b (only a) ==> disjoint b a); admit() *)
-    (* assert(forall (#t:Type) (b:buffer t). (frameOf b = rid /\ live h0 b /\ disjointSet b (only a)) ==> (frameOf b = rid /\ live h0 b /\ disjointSet b (only sub)));  *)
-    (* admit() *)
 
 (* TODO *)
 let modifies_subbuffer_2 (#t:Type) (#t':Type) h0 h1 (sub:buffer t) (a':buffer t') (a:buffer t) : Lemma
-  (requires (live h0 a /\ live h0 a' /\ includes a sub /\ modifies_2 sub a' h0 h1))
+  (requires (live h0 a /\ live h0 a' /\ includes a sub /\ modifies_2 sub a' h0 h1 ))
+  (ensures  (modifies_2 a a' h0 h1 /\ modifies_2 a' a h0 h1 /\ live h1 a))
+  [SMTPat (modifies_2 sub a' h0 h1); SMTPat (includes a sub)]
+  = admit()
+
+let modifies_subbuffer_2' (#t:Type) (#t':Type) h0 h1 (sub:buffer t) (a':buffer t') (a:buffer t) : Lemma
+  (requires (live h0 a /\ live h0 a' /\ includes a sub /\ modifies_2 a' sub h0 h1 ))
   (ensures  (modifies_2 a a' h0 h1 /\ live h1 a))
+  [SMTPat (modifies_2 a' sub h0 h1); SMTPat (includes a sub)]
+  = admit()
+
+let modifies_subbuffer_2_1 (#t:Type) h0 h1 (sub:buffer t) (a:buffer t) : Lemma
+  (requires (live h0 a /\ includes a sub /\ modifies_2_1 sub h0 h1))
+  (ensures  (modifies_2_1 a h0 h1 /\ live h1 a))
+  [SMTPat (modifies_2_1 sub h0 h1); SMTPat (includes a sub)]
+  = admit()
+
+let modifies_subbuffer_2_prime (#t:Type) h0 h1 (sub1:buffer t) (sub2:buffer t) (a:buffer t) : Lemma
+  (requires (live h0 a /\ includes a sub1 /\ includes a sub2 /\ modifies_2 sub1 sub2 h0 h1))
+  (ensures  (modifies_1 a h0 h1 /\ live h1 a))
+  [SMTPat (modifies_2 sub1 sub2 h0 h1); SMTPat (includes a sub1); SMTPat (includes a sub2)]
   = admit()
 
 let modifies_popped_1 (#t:Type) (a:buffer t) h0 h1 h2 h3 : Lemma
   (requires (live h0 a /\ fresh_frame h0 h1 /\ popped h2 h3 /\ modifies_2_1 a h1 h2))
   (ensures  (modifies_1 a h0 h3))
-  [SMTPat (fresh_frame h0 h1 /\ popped h2 h3 /\ modifies_2_1 a h1 h2)]
+  [SMTPat (fresh_frame h0 h1); SMTPat (popped h2 h3); SMTPat (modifies_2_1 a h1 h2)]
+  = ()
+
+let modifies_popped_0 h0 h1 h2 h3 : Lemma
+  (requires (fresh_frame h0 h1 /\ popped h2 h3 /\ modifies_0 h1 h2))
+  (ensures  (modifies_0 h0 h3))
+  [SMTPat (fresh_frame h0 h1); SMTPat (popped h2 h3); SMTPat (modifies_0 h1 h2)]
+  = ()
+
+let modifies_0_to_2_1_lemma (#t:Type) h0 h1 (b:buffer t) : Lemma
+  (requires (modifies_0 h0 h1 /\ live h0 b))
+  (ensures  (modifies_2_1 b h0 h1))
+  [SMTPat (modifies_2_1 b h0 h1); SMTPat (live h0 b) ]
   = ()
